tlb: adding more lifting results and wellformed proofs
Signed-off-by: Reto Achermann <reto.achermann@inf.ethz.ch>

theories/mipstlb/MipsTLBEquivalence.thy
@@ -40,7 +40,7 @@ text "Next we show that for all "
 
     
   
-lemma 
+lemma TLBEquivalence :
     assumes inrange: "vpn < MIPSPT_EntriesMax"
         and inrange2: "as < ASIDMax"
         and cap: "capacity (tlb mpt) > 0"
@@ -62,6 +62,85 @@ proof -
   
   from X0 X1 show ?thesis by(auto)
 qed
-  
-  
+
+definition addr2vpn :: "addr \<Rightarrow> VPN"
+  where "addr2vpn a = ((fst a) mod VASize) div 4096"
+
+definition addr2asid :: "addr \<Rightarrow> ASID"
+  where "addr2asid a = (fst a) div VASize"
+
+definition pfn2addr :: "PFN \<Rightarrow> addr"
+  where "pfn2addr p = (p * 4096, {})"
+
+definition AddrValid :: "addr \<Rightarrow> bool"
+  where "AddrValid a = ((fst a) < VASize * ASIDMax)"
+
+
+lemma AddrValid_implies_inrange :
+  "AddrValid a \<Longrightarrow> addr2vpn a < MIPSPT_EntriesMax"
+  by(auto simp:addr2vpn_def AddrValid_def VASize_def ASIDMax_def MIPSPT_EntriesMax_def)
+
+lemma AddrValid_implies_inrange2 :
+  "AddrValid a \<Longrightarrow> addr2asid a < ASIDMax"
+  by(auto simp:addr2asid_def AddrValid_def VASize_def ASIDMax_def MIPSPT_EntriesMax_def)
+
+
+definition MipsTLBPT_to_node :: "nodeid \<Rightarrow> MipsTLBPT \<Rightarrow> node"
+  where "MipsTLBPT_to_node nid mpt =  \<lparr> accept = {},
+         translate = (\<lambda>a. (if AddrValid a then 
+         (\<Union>x\<in> (MipsTLBPT_translate mpt (addr2asid a) (addr2vpn a)). {(nid, pfn2addr x)} )  else {} ))  \<rparr>"
+
+
+definition MIPSLARGE_to_node :: "nodeid \<Rightarrow> MIPSTLB \<Rightarrow> node"
+  where "MIPSLARGE_to_node nid t =  \<lparr> accept = {},
+        translate = (\<lambda>a.  (if AddrValid a then 
+        (\<Union>x\<in> (MIPSTLB_translate t (addr2asid a) (addr2vpn a)). {(nid, pfn2addr x)} ) else {} ))  \<rparr>"
+
+
+
+lemma Equiv :
+  assumes cap: "capacity (tlb mpt) > 0"
+      and valid: "MipsTLBPT_valid mpt"
+      and avalid: "AddrValid a"
+    shows "(\<Union>x\<in>MipsTLBPT_translate mpt (addr2asid a) (addr2vpn a). {(nid, pfn2addr x)})  = 
+           ( \<Union>x\<in>MIPSTLB_translate (MipsTLBLarge_create (pte mpt)) (addr2asid a) (addr2vpn a). {(nid, pfn2addr x)})"
+proof -
+  from avalid have X0: "addr2asid a < ASIDMax"
+    by(auto simp:AddrValid_implies_inrange2)
+
+  from avalid have X1 : "addr2vpn a < MIPSPT_EntriesMax"
+    by(auto simp:AddrValid_implies_inrange)
+
+  from X0 X1 cap valid show ?thesis
+    by(auto simp: TLBEquivalence)
+qed
+
+
+lemma 
+  assumes cap: "capacity (tlb mpt) > 0"
+      and valid: "MipsTLBPT_valid mpt"
+  shows "MipsTLBPT_to_node nid mpt = 
+         MIPSLARGE_to_node nid (MipsTLBLarge_create (pte mpt))"
+proof -
+  have X0:  "MipsTLBPT_to_node nid mpt =  \<lparr>accept = {}, translate = \<lambda>a. if AddrValid a then \<Union>x\<in>MipsTLBPT_translate mpt (addr2asid a) (addr2vpn a). {(nid, pfn2addr x)} else {}\<rparr>"
+    by(simp add:MipsTLBPT_to_node_def)
+
+  have X1: " MIPSLARGE_to_node nid (MipsTLBLarge_create (pte mpt)) =  \<lparr>accept = {}, translate = \<lambda>a. if AddrValid a then \<Union>x\<in>MIPSTLB_translate (MipsTLBLarge_create (pte mpt)) (addr2asid a) (addr2vpn a). {(nid, pfn2addr x)} else {}\<rparr>"
+    by(simp add:MIPSLARGE_to_node_def)
+
+  from cap valid have X2: "\<And>a. (if AddrValid a then \<Union>x\<in>MipsTLBPT_translate mpt (addr2asid a) (addr2vpn a). {(nid, pfn2addr x)} else {}) = 
+             (if AddrValid a then \<Union>x\<in>MIPSTLB_translate (MipsTLBLarge_create (pte mpt)) (addr2asid a) (addr2vpn a). {(nid, pfn2addr x)} else {})"
+    by(auto simp:Equiv)
+
+
+  from X0 cap valid have X3 :  " \<lparr>accept = {}, translate = \<lambda>a. if AddrValid a then \<Union>x\<in>MipsTLBPT_translate mpt (addr2asid a) (addr2vpn a). {(nid, pfn2addr x)} else {}\<rparr> = 
+                  \<lparr>accept = {}, translate = \<lambda>a. if AddrValid a then \<Union>x\<in>MIPSTLB_translate (MipsTLBLarge_create (pte mpt)) (addr2asid a) (addr2vpn a). {(nid, pfn2addr x)} else {}\<rparr>"
+    by(simp only:X2)
+
+  from X0 X1 X2 show ?thesis by(auto)
+qed
+
+
+
+
 end  
